Coq Proofs

type_members/coq_formalism/type_members.v
@@ -7,6 +7,8 @@ Require Export Arith.
 Inductive var : Type :=
   |v_cons : nat -> var.
 
+Definition self := v_cons 0.
+
 Inductive label : Type :=
   | l_cons : nat -> label.
 
@@ -14,44 +16,52 @@ Inductive label : Type :=
   | m_cons : nat -> meth.*)
 
 Inductive type : Type :=
-  | t_rec   : var -> list type_d -> type
+  | t_rec   : list type_d -> type
   | t_sel   : exp -> label -> type
 (*  | t_union : type -> type -> type*)
   | t_top   : type
   | t_bot   : type
 
 with type_d : Type :=
-  | t_var  : label -> type -> type_d
+  | t_val  : label -> type -> type_d
   | t_def  : label -> type -> type -> type_d
   | t_type : label -> type -> type -> type_d
 
 with exp : Type :=
   | e_var    : var -> exp
-  | e_new    : var -> list decl -> exp -> exp
-  | e_meth   : exp -> label -> exp -> exp
+  | e_loc    : nat -> exp
+  | e_new    : list decl -> exp
+  | e_meth   : exp -> label -> type -> exp -> exp
   | e_field  : exp -> label -> exp
   | e_type   : exp -> type -> exp
 
 with decl : Type :=
-  | d_var  : label -> type -> exp -> decl
+  | d_val  : label -> type -> exp -> decl
   | d_def  : label -> var -> type -> exp -> type -> decl
   | d_type : label -> type -> type -> decl.
 
-Inductive val : exp -> Prop :=
-  | V_Var  : forall x, val (e_var x)
-  | V_Path : forall v f, val v ->
-             val (e_field v f)
-  | V_Type : forall v T, val v ->
-             val (e_type v T).
+Inductive is_path : exp -> Prop :=
+  | P_Var   : forall x, is_path (e_var x)
+  | P_Loc   : forall l, is_path (e_loc l)
+  | P_Field : forall p f, is_path p ->
+              is_path (e_field p f)
+  | P_Type  : forall p T, is_path p ->
+              is_path (e_type p T).
 
-Inductive d_val : decl -> Prop :=
-  | DV_Var : forall f T v,
-             val v ->
-             d_val (d_var f T v)
+Inductive is_value : exp -> Prop :=
+  | V_Loc   : forall l, is_value (e_loc l)
+  | V_Field : forall v f, is_value v ->
+              is_value (e_field v f)
+  | V_Type  : forall v T, is_value v ->
+              is_value (e_type v T).
+
+Inductive is_value_d : decl -> Prop :=
+  | DV_Val : forall f T l,
+             is_value_d (d_val f T (e_loc l))
   | DV_Def : forall m x S e T,
-             d_val (d_def m x S e T)
+             is_value_d (d_def m x S e T)
   | DV_Type : forall L S U,
-             d_val (d_type L S U).
+             is_value_d (d_type L S U).
 
 Fixpoint range {A B : Type} (l: list (A * B)) : list B :=
   match l with
@@ -131,50 +141,50 @@ Fixpoint get {A : Type} (x : var) (l : list (var * A)) : option A :=
   | (y,b)::t => if eq_dec_var x y then Some b else get x t 
 end.
 
-Fixpoint subst_t (x : var) (p : exp) (t : type): type :=
+Fixpoint subst_t (x : var) (v : exp) (t : type): type :=
   match t with
-  | t_rec z D_ => t_rec z (map (subst_D x p) D_)
-  | t_sel p' L => t_sel (subst_e x p p') L
+  | t_rec D_ => t_rec (map (subst_D x v) D_)
+  | t_sel p' L => t_sel (subst_e x v p') L
   | t_top => t
   | t_bot => t
   end
 
-with subst_D (x : var) (p : exp) (D : type_d): type_d :=
+with subst_D (x : var) (v : exp) (D : type_d): type_d :=
   match D with
-  | t_var f T => t_var f (subst_t x p T)
-  | t_def m T T' => t_def m (subst_t x p T) (subst_t x p T')
-  | t_type L T U => t_type L (subst_t x p T) (subst_t x p U)
+  | t_val f T => t_val f (subst_t x v T)
+  | t_def m T T' => t_def m (subst_t x v T) (subst_t x v T')
+  | t_type L T U => t_type L (subst_t x v T) (subst_t x v U)
 end
 
-with subst_e (x : var) (p : exp) (e : exp): exp :=
+with subst_e (x : var) (v : exp) (e : exp): exp :=
   match e with
-  | e_var z => if eq_dec_var x z then p else e
-  | e_new y d_ e' => e_new y (map (subst_d x p) d_) (subst_e x p e')
-  | e_meth e0 m e1 => e_meth (subst_e x p e0) m (subst_e x p e1)
-  | e_field e0 f => e_field (subst_e x p e0) f
-  | e_type e0 T => e_type (subst_e x p e0) T
+  | e_var y => if eq_dec_var x y then v else e
+  | e_loc l => e
+  | e_new d_ => e_new (map (subst_d x v) d_)
+  | e_meth e0 m T e1 => e_meth (subst_e x v e0) m (subst_t x v T) (subst_e x v e1)
+  | e_field e0 f => e_field (subst_e x v e0) f
+  | e_type e0 T => e_type (subst_e x v e0) T
   end
 
-with subst_d (x : var) (p : exp) (d : decl): decl :=
+with subst_d (x : var) (v : exp) (d : decl): decl :=
   match d with
-  | d_var f T e => d_var f (subst_t x p T) (subst_e x p e)
-  | d_def m x T e U => d_def m x (subst_t x p T) (subst_e x p e) (subst_t x p U)
-  | d_type L T U => d_type L (subst_t x p T) (subst_t x p U)
+  | d_val f T e => d_val f (subst_t x v T) (subst_e x v e)
+  | d_def m x T e U => d_def m x (subst_t x v T) (subst_e x v e) (subst_t x v U)
+  | d_type L T U => d_type L (subst_t x v T) (subst_t x v U)
 end.
 
 Inductive notin_e : var -> exp -> Prop :=
   | notin_var : forall x y,
                 x <> y ->
                 notin_e x (e_var y)
-  | notin_new : forall x y d_ e,
+  | notin_new : forall x d_ e,
                 (forall d, In d d_ -> notin_d x d) ->
-                notin_e x (e_var y) ->
                 notin_e x e ->
-                notin_e x (e_new y d_ e)
-  | notin_meth : forall x e m e0,
+                notin_e x (e_new d_)
+  | notin_meth : forall x e m T e0,
                  notin_e x e ->
                  notin_e x e0 ->
-                 notin_e x (e_meth e m e0)
+                 notin_e x (e_meth e m T e0)
   | notin_field : forall x e f,
                  notin_e x e ->
                  notin_e x (e_field e f)
@@ -184,10 +194,10 @@ Inductive notin_e : var -> exp -> Prop :=
                  notin_e x (e_type e T)
 
 with notin_d : var -> decl -> Prop :=
-  | notin_d_var : forall x l T e,
+  | notin_d_val : forall x l T e,
                   notin_t x T ->
                   notin_e x e ->
-                  notin_d x (d_var l T e)
+                  notin_d x (d_val l T e)
   | notin_d_def : forall x m y S e T,
                   notin_t x S ->
                   notin_t x T ->
@@ -199,17 +209,17 @@ with notin_d : var -> decl -> Prop :=
                    notin_d x (d_type L S U)
 
 with notin_t : var -> type -> Prop :=
-  | notin_rec : forall x z D_,
+  | notin_rec : forall x D_,
                 (forall D, In D D_ -> notin_D x D) ->
-                notin_t x (t_rec z D_)
+                notin_t x (t_rec D_)
   | notin_sel : forall x p L,
                 notin_e x p ->
                 notin_t x (t_sel p L)
 
 with notin_D : var -> type_d -> Prop :=
-  | notin_D_var : forall x f T,
+  | notin_D_val : forall x f T,
                    notin_t x T ->
-                   notin_D x (t_var f T)
+                   notin_D x (t_val f T)
   | notin_D_def : forall x m S T,
                    notin_t x S ->
                    notin_t x T ->
@@ -219,150 +229,186 @@ with notin_D : var -> type_d -> Prop :=
                    notin_t x U ->
                    notin_D x (t_type L S U).
 
-Inductive typing : list (var * type) -> exp -> type -> Prop :=
-  | T_Var : forall G x T,
-            In (x,T) G ->
-            typing G (e_var x) T
-
-  | T_New : forall G y d_ e T,
-            (exists2 D_, typings_d ((y, t_rec y D_)::G) d_ D_ &
-                         typing ((y, t_rec y D_)::G) e T) ->
-            ~In y (dom G) ->
-            typing G (e_new y d_ e) T
-
-  | T_Meth : forall G e0 m e1 T0 S T,
-             member G e0 (t_def m S T) ->
-             typing G e0 T0 ->
-             typing G e1 S ->
-             typing G (e_meth e0 m e1) T
-
-  | T_Acc : forall G e0 f T0 T,
-            typing G e0 T0 ->
-            member G e0 (t_var f T) ->
-            typing G (e_field e0 f) T
-
-  | T_Wide : forall G e T,
-             subtyping G e T ->
-             typing G (e_type e T) T
-
-with subtyping : list (var * type) -> exp -> type -> Prop :=
-  | T_Sub : forall G e S T,
-            typing G e S ->
-            sub G S T ->
-            subtyping G e T
-
-with typing_d : list (var * type) -> decl -> type_d -> Prop :=
-  | TD_Var : forall G f T v,
-             typing G v T ->
-             val v ->
-             typing_d G (d_var f T v) (t_var f T)
-
-  | TD_Def : forall G m x S e T,
-             typing ((x,S)::G) e T ->
-             typing_d G (d_def m x S e T) (t_def m S T)
-
-  | TD_Type : forall G L S U,
-              sub G S U ->
-              typing_d G (d_type L S U) (t_type L S U)
-              
-
-with typings_d : list (var * type) -> list decl -> list type_d -> Prop :=
-  | TD_Nil : forall G, typings_d G nil nil
-
-  | TD_Head : forall G d D d_ D_,
-              typing_d G d D ->
-              typings_d G d_ D_ ->
-              typings_d G (d::d_) (D::D_)
-
-with sub : list (var * type) -> type -> type -> Prop :=
-  | S_Refl      : forall G T, sub G T T
-
-  | S_Rec       : forall G z z' D_ D_',
-                  (forall D', In D' D_' -> 
-                  exists2 D, In D D_ & sub_d ((z,t_rec z D_)::G) D (subst_D z' (e_var z) D')) ->
-                  sub G (t_rec z D_) (t_rec z' D_')
-
-  | S_Sel_Upper : forall G p L S U U',
-                  sub G U U' ->
-                  member G p (t_type L S U) ->
-                  sub G (t_sel p L) U'
-
-  | S_Sel_Lower : forall G p L S U S',
-                  sub G S' S ->
-                  member G p (t_type L S U) ->
-                  sub G S' (t_sel p L)
-
-  | S_Top       : forall G T,
-                  sub G T t_top
-
-  | S_Bot       : forall G T,
-                  sub G t_bot T
-
-with sub_d : list (var * type) -> type_d -> type_d -> Prop :=
-  | SD_Var  : forall G f S T,
-              sub G S T ->
-              sub_d G (t_var f S) (t_var f T)
-  | SD_Def  : forall G m S T S' T',
-              sub G S' S ->
-              sub G T T' ->
-              sub_d G (t_def m S T) (t_def m S' T')
-  | SD_Type : forall G L S U S' U',
-              sub G S' S ->
-              sub G U U' ->
-              sub_d G (t_type L S U) (t_type L S' U')
-
-with expansion : list (var * type) -> var -> type -> list type_d -> Prop:=
-  | E_Rec : forall G z D_,
-            expansion G z (t_rec z D_) D_
-  | E_Sel : forall G z p L S U D_,
-            val p ->
-            member G p (t_type L S U) ->
-            expansion G z U D_ ->
-            expansion G z (t_sel p L) D_
-
-with member : list (var * type) -> exp -> type_d -> Prop:=
-  | M_Path : forall G z p T D_ D,
-             typing G p T ->
-             expansion G z T D_ ->
-             In D D_ ->
-             member G p (subst_D z p D)
-  | M_Exp : forall G z e T D_ D,
-            typing G e T ->
-            expansion G z T D_ ->
-            In D D_ ->
-            notin_D z D ->
-            member G e D.
-
-Definition store := list (var * list decl).
-
-Fixpoint lookup {A : Type} (x : var) (u : list (var * A)) : option (var * A) :=
-match u with
+Fixpoint lookup {A : Type} (n : nat) (l : list A) : option A :=
+  match l with
   | nil => None
-  | (y,a)::u' => if (eq_dec_var x y) then Some (y,a) else lookup x u'
+  | h::t => match n with
+            | O => Some h
+            | S m => lookup m t
+            end
 end.
 
-Fixpoint lookup_d (l : label) (d_ : list decl) : option decl :=
+Inductive typing : list (var * type) -> list type -> exp -> type -> Prop :=
+  | T_Var : forall G E x T,
+            In (x,T) G ->
+            typing G E (e_var x) T
+
+  | T_Loc : forall G E l T,
+            lookup l E = Some T ->
+            typing G E (e_loc l) T
+
+  | T_New : forall G E d_ e T,
+            (exists2 D_, typings_d ((self, t_rec D_)::G) E d_ D_ &
+                         typing ((self, t_rec D_)::G) E e T) ->
+            typing G E (e_new d_) T
+
+  | T_Meth : forall G E e0 m U e1 T0 S T,
+             member G E e0 (t_def m S T) ->
+             typing G E e0 T0 ->
+             typing G E e1 S ->
+             sub G E T U ->
+             typing G E (e_meth e0 m U e1) U
+
+  | T_Acc : forall G E e0 f T0 T,
+            typing G E e0 T0 ->
+            member G E e0 (t_val f T) ->
+            typing G E (e_field e0 f) T
+
+  | T_Wide : forall G E e T,
+             subtyping G E e T ->
+             typing G E (e_type e T) T
+
+with subtyping : list (var * type) -> list type -> exp -> type -> Prop :=
+  | T_Sub : forall G E e S T,
+            typing G E e S ->
+            sub G E S T ->
+            subtyping G E e T
+
+with typing_d : list (var * type) -> list type -> decl -> type_d -> Prop :=
+  | TD_Val_x : forall G E f T e,
+             typing G E e T ->
+             typing_d G E (d_val f T e) (t_val f T)
+
+  | TD_Def : forall G E m x S e T,
+             typing ((x,S)::G) E e T ->
+             typing_d G E (d_def m x S e T) (t_def m S T)
+
+  | TD_Type : forall G E L S U,
+              sub G E S U ->
+              typing_d G E (d_type L S U) (t_type L S U)
+
+with typings_d : list (var * type) -> list type -> list decl -> list type_d -> Prop :=
+  | TD_Nil : forall G E, typings_d G E nil nil
+
+  | TD_Head : forall G E d D d_ D_,
+              typing_d G E d D ->
+              typings_d G E d_ D_ ->
+              typings_d G E (d::d_) (D::D_)
+
+with subtyping_d : list (var * type) -> list type -> decl -> type_d -> Prop :=
+  | TD_Sub : forall G E d D D',
+             typing_d G E d D ->
+             sub_d G E D D' ->
+             subtyping_d G E d D'
+
+with subtypings_d : list (var * type) -> list type -> list decl -> list type_d -> Prop :=
+  | Sub_TD_Nil  : forall G E, subtypings_d G E nil nil
+
+  | Sub_TD_Head : forall G E d D d_ D_,
+                  subtyping_d G E d D ->
+                  subtypings_d G E d_ D_ ->
+                  subtypings_d G E (d::d_) (D::D_)
+
+with sub : list (var * type) -> list type -> type -> type -> Prop :=
+  | S_Refl      : forall G E T, sub G E T T
+
+  | S_Rec       : forall G E D_ D_',
+                  subs_d G E D_ D_' ->
+                  sub G E (t_rec D_) (t_rec D_')
+
+  | S_Sel_Upper : forall G E p L S U U',
+                  sub G E U U' ->
+                  member G E p (t_type L S U) ->
+                  sub G E (t_sel p L) U'
+
+  | S_Sel_Lower : forall G E p L S U S',
+                  sub G E S' S ->
+                  member G E p (t_type L S U) ->
+                  sub G E S' (t_sel p L)
+
+  | S_Top       : forall G E T,
+                  sub G E T t_top
+
+  | S_Bot       : forall G E T,
+                  sub G E t_bot T
+
+with sub_d : list (var * type) -> list type -> type_d -> type_d -> Prop :=
+  | SD_Var  : forall G E f S T,
+              sub G E S T ->
+              sub_d G E (t_val f S) (t_val f T)
+  | SD_Def  : forall G E m S T S' T',
+              sub G E S' S ->
+              sub G E T T' ->
+              sub_d G E (t_def m S T) (t_def m S' T')
+  | SD_Type : forall G E L S U S' U',
+              sub G E S' S ->
+              sub G E U U' ->
+              sub_d G E (t_type L S U) (t_type L S' U')
+
+with subs_d : list (var * type) -> list type -> list type_d -> list type_d -> Prop :=
+  | SD_Nil  : forall G E D_,
+              subs_d G E D_ nil
+  | SD_list  : forall G E D_ D_' D D',
+              sub_d G E D D' ->
+              subs_d G E D_ D_' ->
+              subs_d G E (D::D_) (D'::D_')
+
+with expansion : list (var * type) -> list type -> type -> list type_d -> Prop:=
+  | E_Rec : forall G E D_,
+            expansion G E (t_rec D_) D_
+  | E_Sel : forall G E p L S U D_,
+            is_path p ->
+            member G E p (t_type L S U) ->
+            expansion G E U D_ ->
+            expansion G E (t_sel p L) D_
+
+with member : list (var * type) -> list type -> exp -> type_d -> Prop:=
+  | M_Path : forall G E p T D_ D,
+             typing G E p T ->
+             expansion G E T D_ ->
+             In D D_ ->
+             member G E p (subst_D self p D)
+  | M_Exp : forall G E e T D_ D,
+            typing G E e T ->
+            expansion G E T D_ ->
+            In D D_ ->
+            notin_D self D ->
+            member G E e D.
+
+Hint Constructors typing subtyping typing_d typings_d subtyping_d subtypings_d sub sub_d subs_d expansion member.
+
+Inductive sub_t : list (var * type) -> list type -> type -> type -> Prop :=
+  | S_t_Refl  : forall G E T, sub_t G E T T
+  | S_t_Trans : forall G E S T U, sub_t G E S T ->
+                sub G E T U ->
+                sub_t G E S U.
+
+Hint Constructors sub_t.
+
+Definition store := list (list decl).
+
+Fixpoint get_d (l : label) (d_ : list decl) : option decl :=
 match d_ with
   | nil => None
   | d::d_' => match d with
-                | d_var f T e => if (eq_dec_lab l f) then Some d else lookup_d l d_'
-                | d_def m x T e U => if (eq_dec_lab l m) then Some d else lookup_d l d_'
-                | d_type L T U => if (eq_dec_lab l L) then Some d else lookup_d l d_'
+                | d_val f T e => if (eq_dec_lab l f) then Some d else get_d l d_'
+                | d_def m x T e U => if (eq_dec_lab l m) then Some d else get_d l d_'
+                | d_type L T U => if (eq_dec_lab l L) then Some d else get_d l d_'
               end
 end.
 
-Inductive path : exp -> store -> var * list decl -> Prop :=
-  | p_var : forall x u y d_,
-            lookup x u = Some (y,d_) ->
-            path (e_var x) u (y,d_)
-  | p_field : forall e f u x d_ l T v z d_',
-              path (e_field e f) u (x, d_) ->
-              lookup_d f d_ = Some (d_var l T v) ->
-              path v u (z, d_') ->
-              path (e_field e f) u (z, d_')
-  | p_type : forall e T u z d_,
-             path e u (z, d_) ->
-             path (e_type e T) u (z, d_).
+Inductive path : exp -> store -> nat -> Prop :=
+  | p_var   : forall l u,
+              path (e_loc l) u l
+  | p_field : forall e f u l l' d_ f' T v,
+              path e u l' ->
+              lookup l' u = Some d_->
+              get_d f d_ = Some (d_val f' T v) ->
+              path v u l ->
+              path (e_field e f) u l
+  | p_type  : forall e T u l,
+              path e u l ->
+              path (e_type e T) u l.
 
 (*Fixpoint path (e : exp) (u : store) : option (var * list decl) :=
 match e with
@@ -379,6 +425,139 @@ match e with
   | e_type e0 T => path e0 u
   | _ => None
 end.*)
+Require Export String.
+Open Scope string_scope.
+
+Ltac move_to_top x :=
+  match reverse goal with
+  | H : _ |- _ => try move x after H
+  end.
+Tactic Notation "assert_eq" ident(x) constr(v) :=
+  let H := fresh in
+  assert (x = v) as H by reflexivity;
+  clear H.
+
+Tactic Notation "Case_aux" ident(x) constr(name) :=
+  first [
+    set (x := name); move_to_top x
+  | assert_eq x name; move_to_top x
+  | fail 1 "because we are working on a different case" ].
+
+Tactic Notation "Case" constr(name) := Case_aux Case name.
+Tactic Notation "SCase" constr(name) := Case_aux SCase name.
+Tactic Notation "SSCase" constr(name) := Case_aux SSCase name.
+Tactic Notation "SSSCase" constr(name) := Case_aux SSSCase name.
+Tactic Notation "SSSSCase" constr(name) := Case_aux SSSSCase name.
+Tactic Notation "SSSSSCase" constr(name) := Case_aux SSSSSCase name.
+Tactic Notation "SSSSSSCase" constr(name) := Case_aux SSSSSSCase name.
+Tactic Notation "SSSSSSSCase" constr(name) := Case_aux SSSSSSSCase name.
+
+Scheme typing_typing_ind := Minimality for typing Sort Prop
+with typing_subtyping_ind := Minimality for subtyping Sort Prop
+with typing_typing_d_ind := Minimality for typing_d Sort Prop
+with typing_typings_d_ind := Minimality for typings_d Sort Prop
+with typing_subtyping_d_ind := Minimality for subtyping_d Sort Prop
+with typing_subtypings_d_ind := Minimality for subtypings_d Sort Prop
+with typing_sub_ind := Minimality for sub Sort Prop
+with typing_sub_d_ind := Minimality for sub_d Sort Prop
+with typing_subs_d_ind := Minimality for subs_d Sort Prop
+with typing_expansion_ind := Minimality for expansion Sort Prop
+with typing_member_ind := Minimality for member Sort Prop.
+
+Combined Scheme typing_mutind from 
+      typing_typing_ind,
+      typing_subtyping_ind,
+      typing_typing_d_ind,
+      typing_typings_d_ind,
+      typing_subtyping_d_ind,
+      typing_subtypings_d_ind,
+      typing_sub_ind,
+      typing_sub_d_ind,
+      typing_subs_d_ind,
+      typing_expansion_ind,
+      typing_member_ind.
+
+Scheme subtype_sub_ind := Minimality for sub Sort Prop
+with subtype_sub_d_ind := Minimality for sub_d Sort Prop
+with subtype_subs_d_ind := Minimality for subs_d Sort Prop.
+
+Combined Scheme sub_mutind from 
+      subtype_sub_ind,
+      subtype_sub_d_ind,
+      subtype_subs_d_ind.
+
+Notation "l1 '++' l2" := (app l1 l2).
+
+Theorem environment_narrowing_mutind : 
+  (forall G E e T, typing G E e T -> (forall G_a x S U G_b,
+                                      G = (G_a ++ ((x,U)::G_b)) ->
+                                      sub G_a E S U ->
+                                      subtyping (G_a ++ ((x,S)::G_b)) E e T)) /\
+
+  (forall G E e T, subtyping G E e T -> (forall G_a x S U G_b,
+                                         G = (G_a ++ ((x,U)::G_b)) ->
+                                         sub G_a E S U ->
+                                         subtyping (G_a ++ ((x,S)::G_b)) E e T)) /\
+
+  (forall G E d D, typing_d G E d D -> (forall G_a x S U G_b,
+                                         G = (G_a ++ ((x,U)::G_b)) ->
+                                         sub G_a E S U ->
+                                         typing_d (G_a ++ ((x,S)::G_b)) E d D)) /\
+
+  (forall G E d_ D_, typings_d G E d_ D_ -> (forall G_a x S U G_b,
+                                               G = (G_a ++ ((x,U)::G_b)) ->
+                                               sub G_a E S U ->
+                                               subtypings_d (G_a ++ ((x,S)::G_b)) E d_ D_)) /\
+
+  (forall G E d D, subtyping_d G E d D -> (forall G_a x S U G_b,
+                                               G = (G_a ++ ((x,U)::G_b)) ->
+                                               sub G_a E S U ->
+                                               subtyping_d (G_a ++ ((x,S)::G_b)) E d D)) /\
+
+  (forall G E d_ D_, subtypings_d G E d_ D_ -> (forall G_a x S U G_b,
+                                               G = (G_a ++ ((x,U)::G_b)) ->
+                                               sub G_a E S U ->
+                                               subtypings_d (G_a ++ ((x,S)::G_b)) E d_ D_)) /\
+
+  (forall G E T T', sub G E T T' -> (forall G_a x S U G_b,
+                                       G = (app G_a ((x,U)::G_b)) ->
+                                       sub G_a E S U ->
+                                       sub (G_a ++ ((x,S)::G_b)) E T T')) /\
+
+  (forall G E D D', sub_d G E D D' -> (forall G_a x S U G_b,
+                                       G = (G_a ++ ((x,U)::G_b)) ->
+                                       sub G_a E S U ->
+                                       sub_d (G_a ++ ((x,S)::G_b)) E D D')) /\
+
+  (forall G E D_ D_', subs_d G E D_ D_' -> (forall G_a x S U G_b,
+                                       G = (G_a ++ ((x,U)::G_b)) ->
+                                       sub G_a E S U ->
+                                       subs_d (G_a ++ ((x,S)::G_b)) E D_ D_')) /\
+
+  (forall G E T D_, expansion G E T D_ -> (forall G_a x S U G_b,
+                                           G = (G_a ++ ((x,U)::G_b)) ->
+                                           sub G_a E S U ->
+                                           expansion (G_a ++ ((x,S)::G_b)) E T D_)) /\
+
+  (forall G E e D, member G E e D -> (forall G_a x S U G_b,
+                                      G = (G_a ++ ((x,U)::G_b)) ->
+                                      sub G_a E S U ->
+                                      member (G_a ++ ((x,S)::G_b)) E e D)).
+Proof.
+  apply typing_mutind; intros; subst; eauto.
+  Case "T_Var".
+    apply T_Var.
+  Case "T_New".
+  Case "T_Meth".
+  Case "TD_Def".
+Qed.  
+  
+  
+
+Theorem subtype_equality : forall G S T,
+  subtype G S T ->
+  subtype G T S ->
+  
 
 Theorem subtype_transitivity : forall G S T,
   sub G S T ->
